time.rb
@@ -39,7 +39,7 @@ end
 def writeETA(mod, time)
 	rev = `git rev-parse HEAD`
   CSV.open(timefile(mod), "ab") do |csv|
-		  csv << ["#{time}", "#{@hostname}", "#{Time.now.to_i}", "#{rev}"]
+		  csv << ["#{time}", "#{@hostname}", "#{Time.now.to_i}", "#{rev.strip}"]
 	end	
 end	
 
