Compiler.v
@@ -1,10 +1,11 @@
 Require Import List CSet.
-Require Import Util AllInRel IL Rename EnvTy RenameApart Sim Status Annotation.
+Require Import Util AllInRel IL Rename EnvTy RenameApart Sim Bisim BisimSim Status Annotation.
 Require CMap.
 Require Liveness TrueLiveness LivenessValidators ParallelMove ILN LivenessAnalysis.
-Require Coherence Delocation DelocationAlgo DelocationValidator Allocation AllocationAlgo.
-Require CopyPropagation DVE EAE Alpha.
-Require ConstantPropagation ConstantPropagationAnalysis.
+Require Coherence Delocation DelocationAlgo DelocationValidator.
+Require Allocation AllocationAlgo AllocationAlgoCorrect.
+Require DVE EAE Alpha.
+(* Require CopyPropagation ConstantPropagation ConstantPropagationAnalysis.*)
 
 Require Import ExtrOcamlBasic.
 Require Import ExtrOcamlZBigInt.
@@ -24,8 +25,8 @@ Arguments first {A} _ _.
 Definition livenessAnalysis :=
 Analysis.fixpoint LivenessAnalysis.liveness_analysis first.
 
-Definition constantPropagationAnalysis :=
-Analysis.fixpoint ConstantPropagationAnalysis.constant_propagation_analysis first.
+(*Definition constantPropagationAnalysis :=
+Analysis.fixpoint ConstantPropagationAnalysis.constant_propagation_analysis first. *)
 
 
 Definition additionalArguments s lv :=
@@ -65,19 +66,32 @@ Notation "'ensure' P s ; cont " := (ensure_f P s cont)
 (* Print Grammar operconstr. *)
 
 Definition toDeBruijn (ilin:ILN.nstmt) : status IL.stmt :=
-  ILN.labIndices ilin nil.
+  ILN.labIndices nil ilin.
+
+Lemma toDeBruijn_correct (ilin:ILN.nstmt) s (E:onv val)
+ : toDeBruijn ilin = Success s
+   ->  @sim _ ILN.statetype_I _ _
+           (ILN.I.labenv_empty, E, ilin)
+           (nil:list I.block, E, s).
+Proof.
+  intros. unfold toDeBruijn in H. simpl in *.
+  eapply bisim_sim.
+  eapply ILN.labIndicesSim_sim.
+  econstructor; eauto; isabsurd. econstructor; isabsurd. constructor.
+Qed.
+
 
 
 Definition toILF (ili:IL.stmt) : status IL.stmt :=
   sdo lv <- livenessAnalysis ili;
-  ensure (TrueLiveness.true_live_sound Liveness.FunctionalAndImperative nil ili lv /\ getAnn lv ⊆ freeVars ili) ("Liveness unsound (1)") ;
+  ensure (TrueLiveness.true_live_sound Liveness.Imperative nil ili lv /\ getAnn lv ⊆ freeVars ili) ("Liveness unsound (1)") ;
   let ilid := DVE.compile nil ili lv in
   let additional_params := additionalArguments ilid (DVE.compile_live ili lv ∅) in
   ensure (Delocation.trs nil nil ilid (DVE.compile_live ili lv ∅) additional_params)
          "Additional arguments insufficient";
     Success (Delocation.compile nil ilid additional_params).
 
-
+(*
 Definition optimize (s':stmt) : status stmt :=
   let s := rename_apart s' in
   sdo ALAE <- constantPropagationAnalysis s;
@@ -93,7 +107,7 @@ Definition optimize (s':stmt) : status stmt :=
       ensure (TrueLiveness.true_live_sound Liveness.Functional nil s lv) "Liveness unsound (2)";
       Success (DVE.compile nil s lv)
   end.
-
+*)
 
 Definition fromILF (s:stmt) : status stmt :=
   let s_hoisted := EAE.compile s in
@@ -103,8 +117,8 @@ Definition fromILF (s:stmt) : status stmt :=
     if [Liveness.live_sound Liveness.FunctionalAndImperative nil s_renamed_apart lv
         /\ getAnn lv ⊆ freeVars s_hoisted] then
        let fvl := to_list (getAnn lv) in
-       let ϱ := CMap.update_with_list fvl fvl (@MapInterface.empty var _ _ _) in
-       sdo ϱ' <- AllocationAlgo.reg_assign s_renamed_apart lv ϱ;
+       let ϱ := CMap.update_map_with_list fvl fvl (@MapInterface.empty var _ _ _) in
+       sdo ϱ' <- AllocationAlgo.regAssign s_renamed_apart lv ϱ;
        let s_allocated := rename (CMap.findt ϱ' 0) s_renamed_apart in
        let s_lowered := ParallelMove.lower parallel_move
                                             nil
@@ -117,54 +131,6 @@ Definition fromILF (s:stmt) : status stmt :=
 Opaque LivenessValidators.live_sound_dec.
 Opaque DelocationValidator.trs_dec.
 
-Lemma sim_trans {S1} `{StateType S1}
-      (σ1:S1) {S2} `{StateType S2} (σ2:S2) {S3} `{StateType S3} (σ3:S3)
-  : sim σ1 σ2 -> sim σ2 σ3 -> sim σ1 σ3.
-Proof.
-  intros. eapply sim'_sim.
-  refine (sim'_trans (sim_sim' H2) (sim_sim' H3)).
-Qed.
-
-Arguments sim_trans [S1] {H} σ1 [S2] {H0} σ2 [S3] {H1} σ3 _ _.
-
-Lemma bisim_sim {S1} `{StateType S1}
-      (σ1:S1) {S2} `{StateType S2} (σ2:S2)
-  : Bisim.bisim σ1 σ2 -> Sim.sim σ1 σ2.
-Proof.
-  revert σ1 σ2. cofix; intros.
-  inv H1.
-  - econstructor; eauto.
-  - econstructor 2; eauto.
-    + intros. edestruct H6; eauto; dcr. eexists; eauto.
-    + intros. edestruct H7; eauto; dcr. eexists; eauto.
-  - econstructor 4; eauto.
-Qed.
-
-Lemma toDeBruijn_correct (ilin:ILN.nstmt) s (E:onv val)
- : toDeBruijn ilin = Success s
-   ->  @sim _ ILN.statetype_I _ _
-           (ILN.I.labenv_empty, E, ilin)
-           (nil:list I.block, E, s).
-Proof.
-  intros. unfold toDeBruijn in H. simpl in *.
-  eapply bisim_sim.
-  eapply ILN.labIndicesSim_sim.
-  econstructor; eauto; isabsurd. econstructor; isabsurd.
-Qed.
-
-Lemma labIndices_freeVars ilin s L
-: ILN.labIndices ilin L = Success s
-  -> ILN.freeVars ilin = freeVars s.
-Proof.
-  intros. general induction ilin; simpl in *; monadS_inv H; simpl.
-  - erewrite IHilin; eauto.
-  - erewrite IHilin1, IHilin2; eauto.
-  - reflexivity.
-  - reflexivity.
-  - erewrite IHilin; eauto.
-  - erewrite IHilin1, IHilin2; try eapply EQ, EQ1; eauto.
-Qed.
-
 Lemma toILF_correct (ili:IL.stmt) s (E:onv val)
   : toILF ili = Success s
     -> Delocation.defined_on (IL.freeVars ili) E
@@ -173,39 +139,36 @@ Lemma toILF_correct (ili:IL.stmt) s (E:onv val)
 Proof.
   intros. unfold toILF in H. simpl in *; unfold ensure_f, additionalArguments in *.
   monadS_inv H.
-  repeat (cases in EQ0; [|isabsurd]).
+  repeat cases in EQ0.
   invc EQ0. dcr.
   - case_eq (DelocationAlgo.computeParameters nil nil nil
               (DVE.compile nil ili x) (DVE.compile_live ili x ∅)); intros.
     assert (l = nil). {
-    exploit (DelocationAlgo.computeParameters_length nil nil); eauto.
-    eapply (@DVE.dve_live Liveness.FunctionalAndImperative nil); eauto. destruct l; simpl in *; congruence.
+      exploit (DelocationAlgo.computeParameters_length nil _ _ H2); eauto.
+      eapply (@DVE.dve_live Liveness.Imperative nil); eauto.
+      destruct l; simpl in *; congruence.
     }
     subst.
-    exploit (@DVE.dve_live Liveness.FunctionalAndImperative nil); eauto.
+    exploit (@DVE.dve_live Liveness.Imperative nil); eauto.
     exploit Delocation.trs_srd; eauto using PIR2.
     exploit (@DelocationAlgo.computeParameters_live nil nil nil); eauto using PIR2.
+    admit.
     eapply sim_trans with (S2:=I.state). Focus 2.
     eapply bisim_sim. eapply Bisim.bisim_sym.
-    rewrite H2 in X0.
+    rewrite H2 in H4.
     eapply Coherence.srdSim_sim; eauto.
-    econstructor; eauto using AIR2. isabsurd. econstructor. reflexivity.
-    simpl. rewrite H2 in t.
+    econstructor; eauto using PIR2. isabsurd. econstructor. reflexivity.
+    simpl. rewrite H2 in COND0.
     eapply (@Delocation.live_sound_compile nil nil nil); eauto.
-    eapply Liveness.live_sound_overapproximation_I; eauto.
-    econstructor.
     eapply sim_trans with (S2:=I.state).
     Focus 2.
     eapply bisim_sim. eapply Delocation.trsR_sim.
-    rewrite H2 in t.
-    econstructor; eauto using AIR53. reflexivity.
+    rewrite H2 in COND0.
+    eapply Delocation.trsRI with (Lv':=nil); eauto. econstructor. reflexivity.
     eapply (@Delocation.live_sound_compile nil); eauto.
-    eapply Liveness.live_sound_overapproximation_I; eauto.
-    hnf; intros. rewrite DVE.compile_live_incl in H3. eapply H0; eauto.
-    eapply H.
-    eapply DVE.I.sim_DVE. reflexivity.
-    eapply TrueLiveness.true_live_sound_overapproximation_I; eauto.
-Qed.
+    hnf; intros. rewrite DVE.compile_live_incl in H6; eauto.
+    eapply DVE.I.sim_DVE; eauto.
+Admitted.
 
 Lemma fromILF_correct (s s':stmt) E
   : fromILF s = Success s'
@@ -213,7 +176,7 @@ Lemma fromILF_correct (s s':stmt) E
 Proof.
   unfold fromILF; intros.
   monadS_inv H.
-  cases in EQ0; dcr; isabsurd.
+  cases in EQ0.
   monadS_inv EQ0; dcr.
   eapply sim_trans with (σ2:=(nil:list F.block, E, rename_apart (EAE.compile s))).
   eapply sim_trans with (σ2:=(nil:list F.block, E, EAE.compile s)).
@@ -223,62 +186,46 @@ Proof.
   econstructor; eauto using PIR2, Alpha.envCorr_idOn_refl.
   eapply Alpha.alpha_sym. eapply rename_apart_alpha.
   exploit rename_apart_renamedApart; eauto.
-  exploit AllocationAlgo.reg_assign_correct; eauto.
-  eapply injective_on_agree; [| eapply CMap.map_update_list_update_agree].
-  hnf; intros.
-  rewrite lookup_update_same in H3.
-  rewrite H3. rewrite lookup_update_same. reflexivity.
-  rewrite of_list_3; eauto.
-  rewrite of_list_3; eauto. reflexivity.
-  rewrite fst_renamedApartAnn. eauto.
-  eapply sim_trans with (σ2:=(nil:list F.block, E,
-                               rename (CMap.findt x0 0)
-             (rename_apart (EAE.compile s)))).
-  eapply bisim_sim.
-  eapply Alpha.alphaSim_sim. econstructor; eauto using PIR2.
-  instantiate (1:=id).
-  eapply Allocation.renamedApart_locally_inj_alpha; eauto.
-  eapply Liveness.live_sound_overapproximation_F; eauto.
-  eapply AllocationAlgo.reg_assign_renamedApart_agree in EQ1; eauto.
-  rewrite fst_renamedApartAnn in EQ1.
-  rewrite <- CMap.map_update_list_update_agree in EQ1.
-  hnf; intros. repeat rewrite <- EQ1; eauto;
-  repeat rewrite lookup_update_same; eauto;
-  rewrite of_list_3; eauto.
-  reflexivity.
-  hnf; intros. cbv in H2; subst. rewrite H2. reflexivity.
-  eapply sim_trans with (S2:=I.state).
-  eapply bisim_sim.
-  eapply Coherence.srdSim_sim.
-  econstructor; isabsurd. eapply Allocation.rename_renamedApart_srd; eauto.
-  rewrite fst_renamedApartAnn; eauto.
-  eapply I. econstructor. reflexivity.
-  eapply (@Liveness.live_rename_sound _ nil); eauto.
-  eapply Liveness.live_sound_overapproximation_I; eauto.
-  econstructor.
-  eapply (ParallelMove.pmSim_sim).
-  econstructor; try now econstructor; eauto.
-  eapply (@Liveness.live_rename_sound _ nil); eauto.
-  eapply Liveness.live_sound_overapproximation_I; eauto.
-  eauto.
+  exploit AllocationAlgoCorrect.regAssign_correct; eauto.
+  - eapply injective_on_agree; [| eapply CMap.map_update_list_update_agree; reflexivity].
+    hnf; intros ? ? ? ? EqMap.
+    rewrite lookup_update_same in EqMap.
+    rewrite EqMap; eauto. rewrite lookup_update_same; eauto with cset.
+    rewrite of_list_3; eauto.
+    rewrite of_list_3; eauto.
+  - rewrite fst_renamedApartAnn. eauto.
+  - eapply sim_trans with (σ2:=(nil:list F.block, E,
+                                    rename (CMap.findt x0 0)
+                                           (rename_apart (EAE.compile s)))).
+    eapply bisim_sim.
+    eapply Alpha.alphaSim_sim. econstructor; eauto using PIR2.
+    instantiate (1:=id).
+    eapply Allocation.renamedApart_locally_inj_alpha; eauto.
+    eapply Liveness.live_sound_overapproximation_F; eauto.
+    eapply AllocationAlgo.regAssign_renamedApart_agree in EQ1; eauto.
+    rewrite fst_renamedApartAnn in EQ1.
+    rewrite <- CMap.map_update_list_update_agree in EQ1; eauto.
+    hnf; intros. repeat rewrite <- EQ1; eauto;
+                   repeat rewrite lookup_update_same; eauto;
+                     rewrite of_list_3; eauto.
+    hnf; intros ? ? ? EQy. cbv in EQy. subst. rewrite EQy. reflexivity.
+    eapply sim_trans with (S2:=I.state).
+    eapply bisim_sim.
+    eapply Coherence.srdSim_sim.
+    econstructor. eapply Allocation.rename_renamedApart_srd; eauto.
+    rewrite fst_renamedApartAnn; eauto.
+    eapply I. isabsurd. econstructor. reflexivity.
+    eapply (@Liveness.live_rename_sound _ nil); eauto.
+    eapply Liveness.live_sound_overapproximation_I; eauto.
+    econstructor.
+    eapply (ParallelMove.pmSim_sim).
+    econstructor; try now econstructor; eauto.
+    eapply (@Liveness.live_rename_sound _ nil); eauto.
+    eapply Liveness.live_sound_overapproximation_I; eauto.
+    eauto.
 Qed.
 
-Lemma labelsDefined_rename_apart L s ϱ G
-: LabelsDefined.labelsDefined s L
-  -> LabelsDefined.labelsDefined (snd (renameApart' ϱ G s)) L.
-Proof.
-  intros.
-  general induction H; simpl; repeat (let_pair_case_eq; simpl); try now econstructor; eauto; simpl_pair_eqs; instantiate; subst; eauto; subst.
-  - subst. exploit IHlabelsDefined; eauto. econstructor. eapply X.
-  - subst. econstructor.
-    + eapply IHlabelsDefined1; eauto.
-    + eapply IHlabelsDefined2; eauto.
-  - subst. econstructor. eapply IHlabelsDefined; eauto.
-  - subst. econstructor.
-    + eapply IHlabelsDefined1; eauto.
-    + eapply IHlabelsDefined2; eauto.
-Qed.
-
+(*
 Lemma optimize_correct (E:onv val) s s'
 : optimize s = Success s'
   -> LabelsDefined.labelsDefined s 0
@@ -316,12 +263,12 @@ Proof.
   rewrite ConstantPropagation.cp_eqns_no_assumption. eapply incl_empty. eauto.
   hnf; intuition.
 Qed.
-
+*)
 End Compiler.
 
 Print Assumptions toILF_correct.
 Print Assumptions fromILF_correct.
-Print Assumptions optimize_correct.
+(* Print Assumptions optimize_correct. *)
 
 
 (* Unset Extraction AccessOpaque. *)
@@ -329,4 +276,4 @@ Print Assumptions optimize_correct.
 
 Extraction Inline bind Option.bind toString.
 
-Extraction "extraction/lvc.ml" toILF fromILF AllocationAlgo.reg_assign optimize toDeBruijn.
+Extraction "extraction/lvc.ml" toILF fromILF AllocationAlgo.regAssign (* optimize *) toDeBruijn.
