Equiv/BisimSim.v
@@ -1,0 +1,19 @@
+Require Import List.
+Require Export Util Var Val Exp Env Map CSet AutoIndTac IL AllInRel Sawtooth.
+Require Export EventsActivated StateType paco Equiv Bisim Sim.
+
+Set Implicit Arguments.
+Unset Printing Records.
+
+Lemma bisim_sim {S1} `{StateType S1}
+      (σ1:S1) {S2} `{StateType S2} (σ2:S2)
+  : Bisim.bisim σ1 σ2 -> Sim.sim σ1 σ2.
+Proof.
+  revert σ1 σ2. cofix; intros.
+  inv H1.
+  - econstructor; eauto.
+  - econstructor 2; eauto.
+    + intros. edestruct H6; eauto; dcr. eexists; eauto.
+    + intros. edestruct H7; eauto; dcr. eexists; eauto.
+  - econstructor 4; eauto.
+Qed.
